src/Spec/Modules.v
@@ -1,0 +1,53 @@
+Require Import ConcurProc.
+Require Import Equiv.
+Require Import Compile.
+Require Import Abstraction.
+
+
+(** Combining trace matching with state abstraction. *)
+
+Section TraceAbs.
+
+  Variable opLoT : Type -> Type.
+  Variable opMidT : Type -> Type.
+  Variable opHiT : Type -> Type.
+
+  Variable StateLo : Type.
+  Variable StateMid : Type.
+  Variable absR : StateLo -> StateMid -> Prop.
+
+  Variable lo_step : OpSemantics opLoT StateLo.
+  Variable mid_step : OpSemantics opMidT StateMid.
+
+  Definition traces_match_abs
+                           (ts1 : @threads_state opLoT opHiT)
+                           (ts2 : @threads_state opMidT opHiT) :=
+  forall (sl : StateLo) (sm : StateMid) tr1,
+    exec_prefix lo_step sl ts1 tr1 ->
+    absR sl sm ->
+    exists tr2,
+      exec_prefix mid_step sm ts2 tr2 /\
+      trace_match_hi tr1 tr2.
+
+End TraceAbs.
+
+
+Module Type Layer.
+
+  Axiom opT : Type -> Type.
+  Axiom State : Type.
+  Axiom step : OpSemantics opT State.
+
+End Layer.
+
+
+Module Type LayerImpl (l1 : Layer) (l2 : Layer).
+
+  Axiom absR : l1.State -> l2.State -> Prop.
+  Axiom compile_ts :
+    forall l3opT, @threads_state l2.opT l3opT -> @threads_state l1.opT l3opT.
+  Axiom compile_traces_match :
+    forall `(ts2 : @threads_state _ l3opT),
+      traces_match_abs absR l1.step l2.step (compile_ts ts2) ts2.
+
+End LayerImpl.
